start sketching new setup

examples/pseudo_bool/cp_encoding/cp_to_ilpScript.sml
@@ -1,5 +1,5 @@
 (*
-  Formalization of the CP to ILP phase
+  Formalization of the CP to ILP phase (shared infrastructure)
 *)
 Theory cp_to_ilp
 Libs
@@ -7,47 +7,13 @@ Libs
 Ancestors
   cp ilp pbc pbc_encode sptree
 
-(* TODO: copied from npbc_check, move into misc... *)
-Theorem MEM_enumerate_index:
-  ∀k xs.
-  MEM (i,e) (enumerate k xs) ⇒
-  ∃j. j < LENGTH xs ∧ i = k + j
-Proof
-  Induct_on`xs`>>rw[miscTheory.enumerate_def]
-  >- intLib.ARITH_TAC>>
-  first_x_assum drule>>
-  rw[]
-  >- intLib.ARITH_TAC
-QED
-
-Theorem MEM_enumerate_iff:
-  MEM ie (enumerate 0 xs) ⇔
-  ∃i e. ie = (i,e) ∧ i < LENGTH xs ∧ EL i xs = e
-Proof
-  Cases_on`ie`>>
-  rename1`MEM (i,e) _ `>>
-  Cases_on`i < LENGTH xs`>>fs[MEM_enumerate]
-  >- metis_tac[]>>
-  CCONTR_TAC>>fs[]>>
-  drule MEM_enumerate_index>>
-  rw[]
-QED
+(* The shared infrastructure for all encodings goes into this file *)
 
 (* The datatype for reified variables in the ILP encoding *)
 Datatype:
   reif =
   | Ge 'a int (* Reifies X ≥ i *)
   | Eq 'a int (* Reifies X = i *)
-End
-
-(* The datatype for flags in the ILP encoding *)
-Datatype:
-  flag =
-  | Ne ('a + int) ('a + int)  (* Used to force X ≠ Y *)
-  | Gem ('a + int) ('a + int) (* Used to force X ≥ Y in Array Max *)
-  | Eqc ('a + int) ('a + int) (* Used to force X = Y in Count *)
-  | Nv ('a list) int (* Used to force some element in As = v *)
-  | Tb ('a list) (int list)
 End
 
 Definition reify_reif_def:
@@ -57,13 +23,23 @@ Definition reify_reif_def:
   | Eq X i => wi X = i
 End
 
+(* The datatype for flags in the ILP encoding. *)
+Datatype:
+  flag =
+  | Ne ('a + int) ('a + int)  (* Used to force X ≠ Y *)
+  | Gem ('a + int) ('a + int) (* Used to force X ≥ Y in Array Max *)
+  | Eqc ('a + int) ('a + int) (* Used to force X = Y in Count *)
+  | Nv ('a list) int (* Used to force some element in As = v *)
+  | Tb (('a # int) list) (* Forces Xs = t for a given row*)
+End
+
 Definition reify_flag_def:
   reify_flag wi flag ⇔
   case flag of
   | Ne X Y => varc wi X > varc wi Y
   | Gem X Y => varc wi X ≥ varc wi Y
   | Eqc X Y => varc wi X = varc wi Y
-  | Tb Xs Ts => MAP wi Xs = Ts
+  | Tb Xts => EVERY (λ(X,t). wi X = t) Xts
   | Nv Xs v => MEM v $ MAP wi Xs
 End
 
@@ -83,6 +59,7 @@ Definition reify_avar_def:
     INL reif => reify_reif wi reif
   | INR flag => reify_flag wi flag
 End
+
 
 (***
   Helper encoding functions
@@ -162,7 +139,7 @@ Proof
   fs[]
 QED
 
-Theorem FORALL_IMP_EQ[local] = METIS_PROVE []
+Theorem FORALL_IMP_EQ = METIS_PROVE []
   ``(∀x. P x ⇒ (Q x ⇔ R x)) ⇒ ((∀x. P x ⇒ Q x) ⇔ (∀x. P x ⇒ R x))``;
 
 Theorem encode_eqs_sem[simp]:
@@ -200,1126 +177,234 @@ Proof
   intLib.ARITH_TAC
 QED
 
-(* encode the bound 1 ≤ X ≤ n,
-  which commonly occurs when X indexes into an array *)
-Definition encode_properindex_def:
-  encode_properindex bnd n X =
-  let
-    (lb,ub) = bnd X;
-    xlb = if lb < 1 then [([(1i,X)],[],1i)] else [];
-    xub = if &n < ub then [([(-1i,X)],[],-&n)] else [];
-  in
-    xlb ++ xub
+(*
+  General setup for problem encodings from
+  mlstring-variabled CP constraints.
+
+  mlstring constraint
+
+  into
+
+  (mlstring option # (mlstring, cvar) iconstraint)
+
+  where cvar is mlstring reif + num
+
+  The mlstring option is an annotation.
+*)
+
+Type cvar = ``:(mlstring reif + num)``
+Type ciconstraint = ``:(mlstring, cvar) iconstraint``
+
+(* TODO: replace ge/eq with faster representations. *)
+Datatype:
+  enc_conf =
+    <|
+       fresh : num (* The next fresh var names for flags *)
+     ; ge : (mlstring # int list) list
+     ; eq : (mlstring # int list) list
+    |>
 End
 
-Theorem encode_properindex_sem[simp]:
-  valid_assignment bnd wi ⇒
-  EVERY (λx. iconstraint_sem x (wi,wb)) (encode_properindex bnd n X) =
-  (1 ≤ wi X ∧ wi X ≤ &n)
-Proof
-  rw[encode_properindex_def]>>
-  pairarg_tac>>rw[iconstraint_sem_def,eval_ilin_term_def,iSUM_def]>>
-  fs[valid_assignment_def]>>
-  first_x_assum drule>>gvs[]>>
-  intLib.ARITH_TAC
-QED
+Definition next_fresh_def:
+  next_fresh ec =
+  let f = ec.fresh in
+  (f, ec with fresh := f+1)
+End
 
 (***
-  NotEquals
+  Semantic tools
 ***)
 
-Definition encode_not_equals_def:
-  encode_not_equals bnd X Y =
-  [
-    bits_imply bnd [Pos (INR (Ne X Y))] (mk_constraint_ge 1 X (-1) Y 1);
-    bits_imply bnd [Neg (INR (Ne X Y))] (mk_constraint_ge 1 Y (-1) X 1)
-  ]
+Definition agree_on_fl_def:
+  agree_on_fl fl wb wbf ⇔
+  (∀x. wb (INL x) = wbf (INL x)) ∧
+  (∀x y.
+    ALOOKUP fl y = SOME x ⇒
+    wb (INR x) = wbf (INR y))
 End
 
-(* Prove together? Or separate? *)
-Theorem not_equals_sem_aux:
-  (if wb (INR (Ne X Y))
-   then varc wi X > varc wi Y
-   else varc wi Y > varc wi X) ⇒
-  not_equals_sem X Y wi
-Proof
-  simp[not_equals_sem_def]>>
-  rw[]>>
-  intLib.ARITH_TAC
-QED
-
-Theorem IMP_AND_LEFT[local]:
-  (P ⇒ Q) ⇒
-  (P ∧ Q ⇔ P)
-Proof
-  metis_tac[]
-QED
-
-Theorem encode_not_equals_sem:
-  valid_assignment bnd wi ⇒
-  EVERY (λx. iconstraint_sem x (wi,wb)) (encode_not_equals bnd X Y)
-  =
-  (
-  (if wb (INR (Ne X Y))
-   then varc wi X > varc wi Y
-   else varc wi Y > varc wi X) ∧
-  not_equals_sem X Y wi)
-Proof
-  strip_tac>>
-  simp[MATCH_MP IMP_AND_LEFT not_equals_sem_aux]>>
-  simp[encode_not_equals_def]>>
-  rw[]>>
-  intLib.ARITH_TAC
-QED
-
-(***
-  AllDifferent
-***)
-
-Definition encode_all_different_def:
-  encode_all_different bnd As =
-  let len = LENGTH As in
-  FLAT
-  (GENLIST (λi.
-    FLAT (GENLIST (λj.
-    if i < j
-    then encode_not_equals bnd (EL i As) (EL j As)
-    else []) len)) len)
+Definition mods_fl_def:
+  mods_fl fl (n:num) m ⇔
+  ∀x. x ∈ set (MAP FST fl) ⇒
+    n ≤ x ∧ x < m
 End
 
-Theorem all_different_sem_aux:
-  (∀i j. i < j ∧ j < LENGTH As ⇒
-    let X = EL i As in
-    let Y = EL j As in
-    if wb (INR (Ne X Y))
-    then varc wi X > varc wi Y
-    else varc wi Y > varc wi X) ⇒
-  all_different_sem As wi
+Theorem mods_fl_nil[simp]:
+  mods_fl [] a b
 Proof
-  rw[all_different_sem_def,EL_ALL_DISTINCT_EL_EQ]>>
-  Cases_on`n1 = n2`>>simp[]>>
-  wlog_tac `n1 < n2` [`n1`,`n2`]
+  rw[mods_fl_def]
+QED
+
+Theorem mods_fl_sing[simp]:
+  mods_fl [(f, v)] f (f+1)
+Proof
+  rw[mods_fl_def]
+QED
+
+(* lookup for when the given ge for a variable has been encoded *)
+Definition has_ge_def:
+  has_ge Y n ec =
+  case ALOOKUP ec.ge Y of
+    NONE => F
+  | SOME ls => MEM n ls
+End
+
+Definition has_eq_def:
+  has_eq Y n ec =
+  case ALOOKUP ec.eq Y of
+    NONE => F
+  | SOME ls => MEM n ls
+End
+
+Definition good_reif_def:
+  good_reif wbf wi ec ⇔
+  (∀Y n. has_ge Y n ec ⇒ (wbf (INL (Ge Y n)) ⇔ wi Y ≥ n)) ∧
+  (∀Y n. has_eq Y n ec ⇒ (wbf (INL (Eq Y n)) ⇔ wi Y = n))
+End
+
+Theorem good_reif_with_fresh[simp]:
+  good_reif wbf wi (ec with fresh := f) =
+  good_reif wbf wi ec
+Proof
+  rw[good_reif_def,has_ge_def,has_eq_def]
+QED
+
+(* enc_rel, just a shorthand *)
+Definition enc_rel_def:
+  enc_rel fl wi es es' ec ec' ⇔
+  mods_fl fl ec.fresh ec'.fresh ∧
+  ec.fresh ≤ ec'.fresh ∧
+  (∀wbf.
+    EVERY (λx. iconstraint_sem (SND x) (wi,wbf)) (append es) ∧
+    good_reif wbf wi ec ⇒
+    agree_on_fl fl
+      (λx. case x of INL v => wbf (INL v) | INR v => reify_flag wi v) wbf ∧
+    good_reif wbf wi ec') ∧
+  ∀wb wbf.
+  agree_on_fl fl wb wbf ∧
+  good_reif wbf wi ec ⇒
+  (EVERY (λx. iconstraint_sem x (wi,wb)) es' ⇔
+  EVERY (λx. iconstraint_sem (SND x) (wi,wbf))
+    (append es))
+End
+
+Theorem enc_rel_Nil:
+  enc_rel [] wi Nil [] ec ec
+Proof
+  rw[enc_rel_def,agree_on_fl_def]
+QED
+
+Theorem agree_on_fl_mods_fl_append:
+  mods_fl fl1 f1 f1' ∧
+  mods_fl fl2 f1' f2 ⇒
+  (agree_on_fl (fl1++fl2)
+    (wb:mlstring reif + mlstring flag -> bool)
+    (wbf:mlstring reif + num -> bool) ⇔
+    agree_on_fl fl1 wb wbf ∧
+    agree_on_fl fl2 wb wbf)
+Proof
+  rw[mods_fl_def,agree_on_fl_def,ALOOKUP_APPEND]>>
+  iff_tac>>rw[]
   >- (
-    `n2 < n1` by fs[]>>
-    first_x_assum drule_all>>
+    first_x_assum irule>>
+    drule ALOOKUP_MEM>>
+    CCONTR_TAC>>gvs[AllCaseEqs(),ALOOKUP_NONE]>>
+    first_x_assum drule>>
+    gvs[MEM_MAP,PULL_EXISTS]>>
+    first_x_assum drule>>
     simp[])>>
-  first_x_assum drule>>
-  rw[EL_MAP]>>
-  intLib.ARITH_TAC
+  gvs[AllCaseEqs()]
 QED
 
-Theorem encode_all_different_sem:
-  valid_assignment bnd wi ⇒
-  EVERY (λx. iconstraint_sem x (wi,wb)) (encode_all_different bnd As)
-  =
-  (
-  (∀i j. i < j ∧ j < LENGTH As ⇒
-    let X = EL i As in
-    let Y = EL j As in
-    if wb (INR (Ne X Y))
-    then varc wi X > varc wi Y
-    else varc wi Y > varc wi X) ∧
-  all_different_sem As wi)
+Theorem enc_rel_Append:
+  enc_rel fl wi es xs ec ec' ∧
+  enc_rel fl' wi es' xs' ec' ec'' ⇒
+  enc_rel (fl++fl') wi (Append es es') (xs++xs') ec ec''
 Proof
-  simp[MATCH_MP IMP_AND_LEFT all_different_sem_aux]>>
-  rw[encode_all_different_def, EVERY_FLAT, EVERY_GENLIST]>>
-  eq_tac>>rw[]>>
-  gvs[PULL_FORALL]
-  >- (
-    first_x_assum(qspecl_then[`i`,`j`] mp_tac)>>
-    simp[encode_not_equals_sem])>>
   rw[]>>
-  first_x_assum drule_all>>
-  metis_tac[encode_not_equals_sem,not_equals_sem_aux]
-QED
-
-Definition encode_different_row_def:
-  (encode_different_row bnd X [] = []) ∧
-  (encode_different_row bnd X (Y::Ys) =
-    encode_not_equals bnd X Y ++ encode_different_row bnd X Ys)
-End
-
-(* recurrence equation for encode_all_different involving encode_different_row *)
-Theorem encode_all_different_alt:
-  (encode_all_different bnd [] = []) ∧
-  (encode_all_different bnd (A::As) =
-    encode_different_row bnd A As ++ encode_all_different bnd As)
-Proof
-  rw[encode_all_different_def,GENLIST_CONS,combinTheory.o_ABS_L,LT_SUC_LE]>>
-  Induct_on ‘As’>>
-  rw[encode_different_row_def,GENLIST_CONS,combinTheory.o_ABS_L]
-QED
-
-(***
-  Element
-***)
-
-(* X_{=i} ⇒ Ai = R where Ai, R can be Varc *)
-Definition encode_element_eq_def:
-  encode_element_eq bnd R X (i:num,Ai) =
-  [
-    bits_imply bnd [Pos (INL (Eq X (&(i+1))))] (mk_constraint_ge 1 Ai (-1) R 0);
-    bits_imply bnd [Pos (INL (Eq X (&(i+1))))] (mk_constraint_ge 1 R (-1) Ai 0)
-  ]
-End
-
-Theorem encode_element_eq_sem:
-  valid_assignment bnd wi ∧
-  (wb (INL (Eq X &(i+1))) ⇔ wi X = &(i+1))
-  ⇒
-  EVERY (λx. iconstraint_sem x (wi,wb))
-    (encode_element_eq bnd R X (i,Ai))
-  =
-  (wi X = &(i+1) ⇒ varc wi R = varc wi Ai)
-Proof
-  rw[encode_element_eq_def]>>
-  intLib.ARITH_TAC
-QED
-
-(* Adds X ≥ 1, - X ≥ -|As| where needed *)
-Definition encode_element_var_def:
-  encode_element_var (bnd:'a bounds) R X As =
-  let
-    n = LENGTH As
-  in
-    encode_ges bnd X (n + 1) ++ encode_eqs bnd X n ++
-    encode_properindex bnd n X ++
-    FLAT (MAP (encode_element_eq bnd R X) (enumerate 0n As))
-End
-
-Theorem numint_le_2[local]:
-  (Num X ≤ Y ⇒ X ≤ &Y) ∧ (1 ≤ X ∧ X ≤ &Y ⇒ 1 ≤ Num X ∧ Num X ≤ Y)
-Proof
-  intLib.ARITH_TAC
-QED
-
-Theorem varc_INL[local]:
-  varc w (INL x) = w x
-Proof
-  simp[varc_def]
-QED
-
-Theorem encode_element_var_sem:
-  valid_assignment bnd wi
-  ⇒
-  EVERY (λx. iconstraint_sem x (wi,wb)) (encode_element_var bnd R X As)
-  =
-  (
-  (∀i. 1 ≤ i ∧ i ≤ LENGTH As + 1 ⇒
-    (wb (INL (Ge X &i)) ⇔ wi X ≥ &i)) ∧
-  (∀i. 1 ≤ i ∧ i ≤ LENGTH As ⇒
-    (wb (INL (Eq X &i)) ⇔ wi X = &i)) ∧
-  element_sem R (INL X) As wi)
-Proof
-  rw[encode_element_var_def]>>
-  simp[GSYM CONJ_ASSOC]>>
-  ho_match_mp_tac LEFT_AND_CONG >> simp[]>>
-  strip_tac>>
-  ho_match_mp_tac LEFT_AND_CONG >> simp[]>>
-  strip_tac>>
-  simp[element_sem_def]>>
-  simp[EVERY_FLAT,EVERY_MAP,Once EVERY_MEM,MEM_enumerate_iff,PULL_EXISTS,encode_element_eq_sem,varc_INL]>>
-  ho_match_mp_tac LEFT_AND_CONG >>
-  simp[]>>strip_tac>>
-  ho_match_mp_tac LEFT_AND_CONG >>
-  CONJ_TAC >- intLib.ARITH_TAC>>
-  strip_tac>>
-  `∃i. wi X = &(i + 1) ∧ i < LENGTH As` by intLib.ARITH_TAC>>
-  simp[]
-QED
-
-Definition encode_element_const_def:
-  encode_element_const R (X:int) As =
-  if 1 ≤ X ∧ X ≤ &(LENGTH As)
-  then
-    let Ai = EL (Num X -1) As in
-    [mk_constraint_ge 1 Ai (-1) R 0;
-     mk_constraint_ge 1 R (-1) Ai 0]
-  else
-    [([],[],1)]
-End
-
-Theorem encode_element_const_sem:
-  EVERY (λx. iconstraint_sem x (wi,wb)) (encode_element_const R X As)
-  =
-  element_sem R (INR X) As wi
-Proof
-  rw[encode_element_const_def,iconstraint_sem_def,eval_ilin_term_def,iSUM_def,eval_lin_term_def,mk_constraint_ge_sem,element_sem_def]
-  >- (
-    simp[varc_def]>>
-    eq_tac>>rw[]>>
-    intLib.ARITH_TAC)>>
-  fs[varc_def]>>
-  intLib.ARITH_TAC
-QED
-
-Definition encode_element_def:
-  encode_element bnd R X As =
-  case X of
-    INL vX => encode_element_var bnd R vX As
-  | INR cX => encode_element_const R cX As
-End
-
-(* TODO: This seem too precise *)
-Theorem encode_element_sem:
-  valid_assignment bnd wi
-  ⇒
-  EVERY (λx. iconstraint_sem x (wi,wb)) (encode_element bnd R X As)
-  =
-  (
-  (case X of INR _ => T | INL X =>
-  (∀i. 1 ≤ i ∧ i ≤ LENGTH As + 1 ⇒
-    (wb (INL (Ge X &i)) ⇔ wi X ≥ &i)) ∧
-  (∀i. 1 ≤ i ∧ i ≤ LENGTH As ⇒
-    (wb (INL (Eq X &i)) ⇔ wi X = &i))) ∧
-  element_sem R X As wi)
-Proof
-  rw[encode_element_def]>>
-  TOP_CASE_TAC>>gvs[]
-  >- (
-    DEP_REWRITE_TAC[encode_element_var_sem]>>
-    metis_tac[])
-  >>
-    metis_tac[encode_element_const_sem]
-QED
-
-Theorem encode_element_sem_1:
-  valid_assignment bnd wi ∧
-  element_sem R X As wi ⇒
-  EVERY (λx. iconstraint_sem x (wi,reify_avar wi)) (encode_element bnd R X As)
-Proof
-  rw[encode_element_def]>>
-  TOP_CASE_TAC>>gvs[]
-  >- (
-    DEP_REWRITE_TAC [encode_element_var_sem]>>
-    simp[reify_avar_def,reify_reif_def])
-  >>
-    metis_tac[encode_element_const_sem]
-QED
-
-Theorem encode_element_sem_2:
-  valid_assignment bnd wi ∧
-  EVERY (λx. iconstraint_sem x (wi,wb)) (encode_element bnd R X As) ⇒
-  element_sem R X As wi
-Proof
-  rw[encode_element_def]>>
-  every_case_tac>>gvs[]
-  >- (
-    pop_assum mp_tac>>
-    DEP_REWRITE_TAC[encode_element_var_sem]>>
-    simp[])
-  >>
-    metis_tac[encode_element_const_sem]
-QED
-
-(***
-  Element2D
-***)
-
-(* encode_element2d for constant X and variable Y *)
-Definition encode_element2d_cv_def:
-  encode_element2d_cv bnd R X Y Tss =
-  if EVERY (λTs. LENGTH Ts = LENGTH $ HD Tss) Tss ∧
-      1 ≤ X ∧ X ≤ &LENGTH Tss
-  then encode_element_var bnd R Y $ EL (Num X - 1) Tss
-  else [([],[],1)]
-End
-
-Theorem encode_element2d_cv_sem:
-  valid_assignment bnd wi ⇒
-  EVERY (λx. iconstraint_sem x (wi,wb)) (encode_element2d_cv bnd R X Y Tss) = (
-  (∀j. 1 ≤ j ∧ j ≤ LENGTH (HD Tss) + 1 ⇒ (wb (INL (Ge Y (&j))) ⇔ wi Y ≥ &j)) ∧
-  (∀j. 1 ≤ j ∧ j ≤ LENGTH (HD Tss) ⇒ (wb (INL (Eq Y (&j))) ⇔ wi Y = &j)) ∧
-  element2d_sem R (INR X) (INL Y) Tss wi)
-Proof
-  strip_tac>>
-  simp[encode_element2d_cv_def,element2d_sem_def]>>
-  reverse IF_CASES_TAC
-  >- (
-    fs[iconstraint_sem_def,EXISTS_MEM,varc_def]
-    >- metis_tac[]>>
-    CCONTR_TAC>>fs[]>>
-    intLib.ARITH_TAC)>>
-  fs[encode_element_var_sem,varc_def,element_sem_def,EVERY_EL]>>
-  `∃i. X = &(i + 1) ∧ i < LENGTH Tss` by
-    (qpat_x_assum`!n. _` kall_tac>>
-    intLib.ARITH_TAC)>>
-  simp[]
-QED
-
-(* encode_element2d for variable X and constant Y *)
-Definition encode_element2d_vc_def:
-  encode_element2d_vc bnd R X Y Tss =
-  if EVERY (λTs. LENGTH Ts = LENGTH $ HD Tss) Tss ∧ 0 < LENGTH Tss ∧
-    1 ≤ Y ∧ Y ≤ &(LENGTH $ HD Tss)
-  then encode_element_var bnd R X $ MAP (EL (Num Y - 1)) Tss
-  else [([],[],1)]
-End
-
-Theorem EL_LIST2D:
-  m < LENGTH ls ⇒ EL m (MAP (EL n) ls) = EL n (EL m ls)
-Proof
-  strip_tac>>
-  irule EL_MAP>>
-  simp[]
-QED
-
-Theorem encode_element2d_vc_sem:
-  valid_assignment bnd wi ⇒
-  EVERY (λx. iconstraint_sem x (wi,wb)) (encode_element2d_vc bnd R X Y Tss) = (
-  (∀i. 1 ≤ i ∧ i ≤ LENGTH Tss + 1 ⇒ (wb (INL (Ge X (&i))) ⇔ wi X ≥ &i)) ∧
-  (∀i. 1 ≤ i ∧ i ≤ LENGTH Tss ⇒ (wb (INL (Eq X (&i))) ⇔ wi X = &i)) ∧
-  element2d_sem R (INL X) (INR Y) Tss wi)
-Proof
-  strip_tac>>
-  simp[encode_element2d_vc_def,element2d_sem_def]>>
-  reverse IF_CASES_TAC
-  >- (
-    fs[iconstraint_sem_def,EXISTS_MEM,varc_def]
-    >- metis_tac[]>>
-    CCONTR_TAC>>fs[]>>
-    intLib.ARITH_TAC)>>
-  fs[encode_element_var_sem,varc_def,element_sem_def,EVERY_EL]>>
-  `∃i. Y = &(i + 1) ∧ i < LENGTH (HD Tss)` by
-    (qpat_x_assum`!n. _` kall_tac>>
-    intLib.ARITH_TAC)>>
-  simp[]>>
-  rpt(match_mp_tac LEFT_AND_CONG>>simp[]>>strip_tac)>>
-  DEP_REWRITE_TAC[EL_MAP]>>simp[]
-QED
-
-(* encode_element2d for constant X and constant Y *)
-Definition encode_element2d_cc_def:
-  encode_element2d_cc bnd R X Y Tss =
-  if EVERY (λTs. LENGTH Ts = LENGTH $ HD Tss) Tss ∧
-    1 ≤ X ∧ X ≤ &LENGTH Tss ∧ 1 ≤ Y ∧ Y ≤ &(LENGTH $ HD Tss)
-  then [
-    mk_constraint_ge 1 (EL (Num Y - 1) $ EL (Num X - 1) Tss) (-1) R 0;
-    mk_constraint_ge 1 R (-1) (EL (Num Y - 1) $ EL (Num X - 1) Tss) 0]
-  else [([],[],1)]
-End
-
-Theorem encode_element2d_cc_sem:
-  EVERY (λx. iconstraint_sem x (wi,wb)) (encode_element2d_cc bnd R X Y Tss) =
-  element2d_sem R (INR X) (INR Y) Tss wi
-Proof
-  rw[encode_element2d_cc_def,element2d_sem_def,varc_def,iconstraint_sem_def]
-  >-intLib.ARITH_TAC>>
-  metis_tac[numint_le_2,GSYM NOT_EVERY]
-QED
-
-Definition encode_element2d_eq_def:
-  encode_element2d_eq bnd R X Y (i:num,j:num,Aij) = [
-    bits_imply bnd [Pos (INL (Eq X &(i + 1))); Pos (INL (Eq Y &(j + 1)))]
-      (mk_constraint_ge 1 Aij (-1) R 0);
-    bits_imply bnd [Pos (INL (Eq X &(i + 1)));Pos (INL (Eq Y &(j + 1)))]
-      (mk_constraint_ge 1 R (-1) Aij 0)]
-End
-
-Theorem encode_element2d_eq_sem:
-  valid_assignment bnd wi ∧
-  (wb (INL (Eq X &(i + 1))) ⇔ wi X = &(i + 1)) ∧
-  (wb (INL (Eq Y &(j + 1))) ⇔ wi Y = &(j + 1)) ⇒
-  EVERY (λx. iconstraint_sem x (wi,wb)) (encode_element2d_eq bnd R X Y (i,j,Aij)) = (
-    wi X = &(i + 1) ∧ wi Y = &(j + 1) ⇒ varc wi R = varc wi Aij)
-Proof
-  rw[encode_element2d_eq_def,iconstraint_sem_def]>>
-  intLib.ARITH_TAC
-QED
-
-(* encode_element2d for variable X and variable Y *)
-Definition encode_element2d_vv_def:
-  encode_element2d_vv bnd R X Y Tss =
-  let
-    n = LENGTH Tss
-  in
-    if 0 < n ∧ EVERY (λTs. LENGTH Ts = LENGTH $ HD Tss) Tss
-    then
-      let
-        m = LENGTH $ HD Tss;
-        mat = enumerate 0 $ MAP (λTs. enumerate 0 Ts) Tss
-      in
-        encode_ges bnd X (n + 1) ++ encode_ges bnd Y (m + 1) ++
-        encode_eqs bnd X n ++ encode_eqs bnd Y m ++
-        encode_properindex bnd n X ++ encode_properindex bnd m Y ++
-        (FLAT $ MAP (λ(i,vec).
-          FLAT $ MAP (λp. encode_element2d_eq bnd R X Y (i,p)) vec) mat)
-    else [([],[],1)]
-End
-
-Theorem EVERY_enumerate2d[local]:
-  0 < LENGTH Tss ∧ EVERY (λTs. LENGTH Ts = LENGTH (HD Tss)) Tss ⇒
-  EVERY (λp. EVERY (λq. R (FST p) q) (SND p))
-    (enumerate 0 (MAP (λTs. enumerate 0 Ts) Tss)) = (
-  ∀i j. i < LENGTH Tss ∧ j < LENGTH (HD Tss) ⇒
-    R i (j, EL j $ EL i Tss))
-Proof
-  strip_tac>>
-  simp[EVERY_MEM,MEM_enumerate_iff,EL_MAP,PULL_EXISTS]>>
-  fs[EVERY_EL]>>
-  metis_tac[]
-QED
-
-Theorem encode_element2d_vv_sem:
-  valid_assignment bnd wi ⇒
-  EVERY (λx. iconstraint_sem x (wi,wb)) (encode_element2d_vv bnd R X Y Tss) = (
-    (∀i. 1 ≤ i ∧ i ≤ LENGTH Tss + 1 ⇒ (wb (INL (Ge X &i)) ⇔ wi X ≥ &i)) ∧
-    (∀j. 1 ≤ j ∧ j ≤ LENGTH (HD Tss) + 1 ⇒ (wb (INL (Ge Y &j)) ⇔ wi Y ≥ &j)) ∧
-    (∀i. 1 ≤ i ∧ i ≤ LENGTH Tss ⇒ (wb (INL (Eq X &i)) ⇔ wi X = &i)) ∧
-    (∀j. 1 ≤ j ∧ j ≤ LENGTH (HD Tss) ⇒ (wb (INL (Eq Y &j)) ⇔ wi Y = &j)) ∧
-    element2d_sem R (INL X) (INL Y) Tss wi)
-Proof
-  reverse $ rw[encode_element2d_vv_def]
-  >-
-    fs[iconstraint_sem_def,element2d_sem_def]>>
-  simp[GSYM CONJ_ASSOC]>>
-  ho_match_mp_tac LEFT_AND_CONG >> simp[]>> strip_tac>>
-  ho_match_mp_tac LEFT_AND_CONG >> simp[]>> strip_tac>>
-  ho_match_mp_tac LEFT_AND_CONG >> simp[]>> strip_tac>>
-  ho_match_mp_tac LEFT_AND_CONG >> simp[]>> strip_tac>>
-  simp[element2d_sem_def,varc_INL]>>
-  ho_match_mp_tac LEFT_AND_CONG >> simp[]>> strip_tac>>
-  ho_match_mp_tac LEFT_AND_CONG >> simp[]>>
-  CONJ_TAC >- intLib.ARITH_TAC>>
-  strip_tac>>
-  ho_match_mp_tac LEFT_AND_CONG >> simp[]>> strip_tac>>
-  ho_match_mp_tac LEFT_AND_CONG >> simp[]>>
-  CONJ_TAC >- intLib.ARITH_TAC>>
-  strip_tac>>
-  simp[EVERY_FLAT,EVERY_MAP,iterateTheory.LAMBDA_PAIR] >>
-  DEP_REWRITE_TAC[EVERY_enumerate2d]>>
-  fs[encode_element2d_eq_sem]>>
-  `∃i j. wi X = &(i + 1) ∧ i < LENGTH Tss ∧
-    wi Y = &(j + 1) ∧ j < LENGTH (HD Tss)` by
-    intLib.ARITH_TAC>>
-  simp[]
-QED
-
-Definition encode_element2d_def:
-  encode_element2d bnd R X Y Tss =
-  case (X,Y) of
-    (INL vX,INL vY) => encode_element2d_vv bnd R vX vY Tss
-  | (INL vX,INR cY) => encode_element2d_vc bnd R vX cY Tss
-  | (INR cX,INL vY) => encode_element2d_cv bnd R cX vY Tss
-  | (INR cX,INR cY) => encode_element2d_cc bnd R cX cY Tss
-End
-
-Theorem encode_element2d_sem:
-  valid_assignment bnd wi ⇒
-  EVERY (λx. iconstraint_sem x (wi,wb)) (encode_element2d bnd R X Y Tss) = (
-    (case X of INR _ => T | INL X' =>
-      (∀i. 1 ≤ i ∧ i ≤ LENGTH Tss + 1 ⇒ (wb (INL (Ge X' (&i))) ⇔ wi X' ≥ &i)) ∧
-      (∀i. 1 ≤ i ∧ i ≤ LENGTH Tss ⇒ (wb (INL (Eq X' (&i))) ⇔ wi X' = &i))) ∧
-    (case Y of INR _ => T | INL Y' =>
-      (∀j. 1 ≤ j ∧ j ≤ LENGTH (HD Tss) + 1 ⇒ (wb (INL (Ge Y' (&j))) ⇔ wi Y' ≥ &j)) ∧
-      (∀j. 1 ≤ j ∧ j ≤ LENGTH (HD Tss) ⇒ (wb (INL (Eq Y' (&j))) ⇔ wi Y' = &j))) ∧
-    element2d_sem R X Y Tss wi)
-Proof
-  rw[encode_element2d_def]>>
-  TOP_CASE_TAC
-  >-(
-    TOP_CASE_TAC
-    >-(
-      simp[encode_element2d_vv_sem]>>
-      metis_tac[])>>
-    simp[encode_element2d_vc_sem]>>
-    metis_tac[])
-  >-(
-    TOP_CASE_TAC
-    >-(
-      simp[encode_element2d_cv_sem]>>
-      metis_tac[])>>
-    simp[encode_element2d_cc_sem])
-QED
-
-(***
-  Abs
-***)
-
-(* Encoding for Y a variable *)
-Definition encode_abs_var_body_def:
-  encode_abs_var_body bnd X Y =
-  let vY = INL Y in
-  [
-    bits_imply bnd [Pos (INL (Ge Y 0))] (mk_constraint_ge 1 X (-1) vY 0);
-    bits_imply bnd [Pos (INL (Ge Y 0))] (mk_constraint_ge 1 vY (-1) X 0);
-    bits_imply bnd [Neg (INL (Ge Y 0))] (mk_constraint_ge 1 X 1 vY 0);
-    bits_imply bnd [Neg (INL (Ge Y 0))] (mk_constraint_ge (-1) X (-1) vY 0);
-  ]
-End
-
-Definition encode_abs_var_def:
-  encode_abs_var bnd X Y =
-  encode_ge bnd Y 0 ++
-  encode_abs_var_body bnd X Y
-End
-
-Theorem encode_abs_var_sem:
-  valid_assignment bnd wi
-  ⇒
-  EVERY (λx. iconstraint_sem x (wi,wb)) (encode_abs_var bnd X Y)
-  =
-  (
-    (wb (INL (Ge Y 0)) ⇔ wi Y ≥ 0) ∧
-    abs_sem X (INL Y) wi
-  )
-Proof
-  rw[encode_abs_var_def,encode_abs_var_body_def]>>
-  match_mp_tac LEFT_AND_CONG>>
-  CONJ_TAC >- simp[encode_ge_sem]>>
-  strip_tac>>
-  simp[bits_imply_sem,mk_constraint_ge_sem,abs_sem_def]>>
-  `varc wi (INL Y) = wi Y` by simp[varc_def]>>
-  intLib.ARITH_TAC
-QED
-
-Definition encode_abs_const_def:
-  encode_abs_const X Y =
-  if Y ≥ 0 then
-  [
-    mk_constraint_ge 1 X (-1) (INR Y) 0;
-    mk_constraint_ge (-1) X 1 (INR Y) 0;
-  ]
-  else
-  [
-    mk_constraint_ge 1 X 1 (INR Y) 0;
-    mk_constraint_ge (-1) X (-1) (INR Y) 0;
-  ]
-End
-
-Theorem encode_abs_const_sem:
-  EVERY (λx. iconstraint_sem x (wi,wb)) (encode_abs_const X Y)
-  =
-  abs_sem X (INR Y) wi
-Proof
-  rw[encode_abs_const_def]>>
-  simp[abs_sem_def,mk_constraint_ge_sem]>>
-  `varc wi (INR Y) = Y` by simp[varc_def]>>
-  simp[]>>
-  intLib.ARITH_TAC
-QED
-
-Definition encode_abs_def:
-  encode_abs bnd X Y =
-  case Y of
-    INL vY => encode_abs_var bnd X vY
-  | INR cY => encode_abs_const X cY
-End
-
-Theorem encode_abs_sem:
-  valid_assignment bnd wi
-  ⇒
-  EVERY (λx. iconstraint_sem x (wi,wb)) (encode_abs bnd X Y)
-  =
-  (
-  (case Y of INR _ => T | INL Y =>
-  (wb (INL (Ge Y 0)) ⇔ wi Y ≥ 0)) ∧
-  abs_sem X Y wi)
-Proof
-  rw[encode_abs_def]>>
-  TOP_CASE_TAC>>gvs[]
-  >-
-    metis_tac[encode_abs_var_sem]
-  >>
-    metis_tac[encode_abs_const_sem]
-QED
-
-(***
-  Ilc
-***)
-
-Definition split_iclin_term_def:
-  (split_iclin_term ([]:'a iclin_term)
-    (acc:'a ilin_term) rhs = (acc,rhs)) ∧
-  (split_iclin_term ((c,X)::xs) acc rhs =
-    case X of
-      INL v => split_iclin_term xs ((c,v)::acc) rhs
-    | INR cc =>
-      split_iclin_term xs acc (rhs - c * cc))
-End
-
-Theorem split_iclin_term_sound:
-  ∀Xs rhs acc xs rhs'.
-    split_iclin_term Xs acc rhs = (xs,rhs') ⇒
-    eval_iclin_term wi Xs + eval_ilin_term wi acc - rhs =
-    eval_ilin_term wi xs - rhs'
-Proof
-  Induct
-  >-simp[split_iclin_term_def, eval_iclin_term_def, eval_ilin_term_def, iSUM_def]
-  >-(
-    Cases>>
-    Cases_on ‘r’>>
-    rw[split_iclin_term_def]>>
-    last_x_assum $ drule_then mp_tac>>
-    rw[eval_iclin_term_def, eval_ilin_term_def, iSUM_def, varc_def]>>
-    intLib.ARITH_TAC)
-QED
-
-Definition encode_ilc_def:
-  encode_ilc (Xs:'a iclin_term) (op:pbop) (rhs:int) =
-  let (xs,rhs) = split_iclin_term Xs [] rhs in
-  case op of
-    GreaterEqual => [(xs, [], rhs)]
-  | Greater => [(xs, [] , rhs+1)]
-  | LessEqual => [(MAP (λ(x:int, y). (-x, y)) xs, [], -rhs)]
-  | Less => [(MAP (λ(x:int, y). (-x, y)) xs, [], -rhs+1)]
-  | Equal => [(xs, [], rhs); (MAP (λ(x:int, y). (-x, y)) xs, [], -rhs)]
-End
-
-Theorem encode_ilc_sem:
-  EVERY (λx. iconstraint_sem x (wi,wb)) (encode_ilc Xs op rhs)
-  ⇔
-  ilc_sem Xs op rhs wi
-Proof
-  rw[encode_ilc_def,ilc_sem_def]>>
-  pairarg_tac>>gvs[]>>
-  CASE_TAC>>
-  simp[iconstraint_sem_def]>>
-  ‘∀xs. eval_ilin_term wi (MAP (λ(x,y). (-x,y)) xs) = -(eval_ilin_term wi xs)’ by (
-    Induct
-    >-simp[eval_ilin_term_def, iSUM_def]
-    >-(
-      Cases>>
-      pop_assum mp_tac>>
-      simp[eval_ilin_term_def, iSUM_def]>>
-      intLib.ARITH_TAC))>>
-  pop_assum (fn thm => simp[thm])>>
-  drule_then (qspec_then ‘wi’ mp_tac) split_iclin_term_sound>>
-  rw[]>>
-  intLib.ARITH_TAC
-QED
-
-(***
-  ArrMax
-***)
-
-(* Encodes that all As ≥ M *)
-Definition encode_Gem_ge_def:
-  encode_Gem_ge bnd As M =
-  MAP (λA. bits_imply bnd [Pos (INR (Gem A M))] (mk_constraint_ge 1 A (-1) M 0)) As
-End
-
-(* iff versions *)
-Definition encode_Gem_ge_iff_def:
-  encode_Gem_ge_iff bnd As M =
-  encode_Gem_ge bnd As M ++
-  MAP (λA. bits_imply bnd [Neg (INR (Gem A M))] (mk_constraint_ge 1 M (-1) A 1)) As
-End
-
- (* Encodes that all As ≤ M *)
-Definition encode_Gem_le_def:
-  encode_Gem_le bnd As M =
-  MAP (λA. bits_imply bnd [Pos (INR (Gem M A))] (mk_constraint_ge 1 M (-1) A 0)) As
-End
-
-Definition encode_Gem_le_iff_def:
-  encode_Gem_le_iff bnd As M =
-  encode_Gem_le bnd As M ++
-  MAP (λA. bits_imply bnd [Neg (INR (Gem M A))] (mk_constraint_ge 1 A (-1) M 1)) As
-End
-
-Theorem encode_Gem_ge_sem:
-  valid_assignment bnd wi ⇒
-  EVERY (λx. iconstraint_sem x (wi,wb)) (encode_Gem_ge bnd As M) =
-    (∀A. MEM A As ∧ wb (INR (Gem A M)) ⇒ varc wi A ≥ varc wi M)
-Proof
-  rw[encode_Gem_ge_def]>>
-  simp[EVERY_MAP,EVERY_MEM,AND_IMP_INTRO]>>
-  ho_match_mp_tac FORALL_IMP_EQ >>rw[]>>
-  intLib.ARITH_TAC
-QED
-
-Theorem encode_Gem_le_sem:
-  valid_assignment bnd wi ⇒
-  EVERY (λx. iconstraint_sem x (wi,wb)) (encode_Gem_le bnd As M) =
-    (∀A. MEM A As ∧ wb (INR (Gem M A)) ⇒ varc wi A ≤ varc wi M)
-Proof
-  rw[encode_Gem_le_def]>>
-  simp[EVERY_MAP,EVERY_MEM,AND_IMP_INTRO]>>
-  ho_match_mp_tac FORALL_IMP_EQ >>rw[]>>
-  intLib.ARITH_TAC
-QED
-
-Theorem encode_Gem_ge_iff_sem:
-  valid_assignment bnd wi ⇒
-  EVERY (λx. iconstraint_sem x (wi,wb)) (encode_Gem_ge_iff bnd As M) =
-    (∀A. MEM A As ⇒ (wb (INR (Gem A M)) ⇔ varc wi A ≥ varc wi M))
-Proof
-  rw[encode_Gem_ge_iff_def,encode_Gem_ge_sem]>>
-  simp[EVERY_MAP,EVERY_MEM,AND_IMP_INTRO]>>
-  simp[intLib.ARITH_PROVE ``X + -1 * (Y:int) ≥ 1 ⇔ ¬ (Y ≥ X)``]>>
-  metis_tac[]
-QED
-
-Theorem encode_Gem_le_iff_sem:
-  valid_assignment bnd wi ⇒
-  EVERY (λx. iconstraint_sem x (wi,wb)) (encode_Gem_le_iff bnd As M) =
-    (∀A. MEM A As ⇒ (wb (INR (Gem M A)) ⇔ varc wi A ≤ varc wi M))
-Proof
-  rw[encode_Gem_le_iff_def,encode_Gem_le_sem]>>
-  simp[EVERY_MAP,EVERY_MEM,AND_IMP_INTRO]>>
-  simp[intLib.ARITH_PROVE ``X + -1 * (Y:int) ≥ 1 ⇔ ¬ (X <= Y)``]>>
-  metis_tac[]
-QED
-
-Definition encode_arr_max_def:
-  encode_arr_max bnd M As =
-  ([], MAP (λA. (1, Pos (INR (Gem A M)))) As, 1) ::
-  encode_Gem_ge bnd As M ++
-  MAP (λA. mk_constraint_ge 1 M (-1) A 0) As
-End
-
-Theorem encode_arr_max_sem:
-  valid_assignment bnd wi ⇒
-  EVERY (λx. iconstraint_sem x (wi,wb)) (encode_arr_max bnd M As) = (
-    (∃A. MEM A As ∧ wb (INR (Gem A M))) ∧
-    (∀A. MEM A As ∧ wb (INR (Gem A M)) ⇒ varc wi A ≥ varc wi M) ∧
-    arr_max_sem M As wi)
-Proof
-  strip_tac>>
-  simp[encode_arr_max_def,encode_Gem_ge_sem]>>
-  match_mp_tac LEFT_AND_CONG>>
-  CONJ_TAC >-
-    simp[iconstraint_sem_def,eval_ilin_term_def,iSUM_def,eval_lin_term_ge_1]>>
-  strip_tac>>
-  match_mp_tac LEFT_AND_CONG>> simp[]>>
-  strip_tac>>
-  simp[arr_max_sem_def,EVERY_MAP,mk_constraint_ge_sem,GSYM integerTheory.INT_POLY_CONV_rth,
-       integerTheory.INT_GE,integerTheory.INT_SUB_LE,MEM_MAP,EVERY_MEM]>>
-  iff_tac>>
-  rw[]>>
-  pop_assum drule>>
-  pop_assum drule>>
-  rw[integerTheory.INT_GE,GSYM integerTheory.INT_LE_ANTISYM]>>
-  simp[SF SFY_ss]
-QED
-
-(***
-  ArrMin
-***)
-
-Definition encode_arr_min_def:
-  encode_arr_min bnd M As =
-  ([], MAP (λA. (1, Pos (INR (Gem M A)))) As, 1) ::
-  encode_Gem_le bnd As M ++
-  MAP (λA. mk_constraint_ge 1 A (-1) M 0) As
-End
-
-Theorem encode_arr_min_sem:
-  valid_assignment bnd wi ⇒
-  EVERY (λx. iconstraint_sem x (wi,wb)) (encode_arr_min bnd M As) = (
-    (∃A. MEM A As ∧ wb (INR (Gem M A))) ∧
-    (∀A. MEM A As ∧ wb (INR (Gem M A)) ⇒ varc wi A ≤ varc wi M) ∧
-    arr_min_sem M As wi)
-Proof
-  strip_tac>>
-  simp[encode_arr_min_def,encode_Gem_le_sem]>>
-  match_mp_tac LEFT_AND_CONG>>
-  CONJ_TAC >-
-    simp[iconstraint_sem_def,eval_ilin_term_def,iSUM_def,eval_lin_term_ge_1]>>
-  strip_tac>>
-  match_mp_tac LEFT_AND_CONG>> simp[]>>
-  strip_tac>>
-  simp[arr_min_sem_def,EVERY_MAP,mk_constraint_ge_sem,GSYM integerTheory.INT_POLY_CONV_rth,
-       integerTheory.INT_GE,integerTheory.INT_SUB_LE,MEM_MAP,EVERY_MEM]>>
-  iff_tac>>
-  rw[]>>
-  pop_assum drule>>
-  pop_assum drule>>
-  rw[integerTheory.INT_GE,GSYM integerTheory.INT_LE_ANTISYM]>>
-  simp[SF SFY_ss]
-QED
-
-(***
-  Count
-***)
-
-Definition encode_count_def:
-  encode_count bnd Y C As =
-  let
-    ilpc =
-    case C of
-      INL vC => [
-        ([(-1, vC)], MAP (λA. (1, Pos (INR (Eqc A Y)))) As, 0);
-        ([(1, vC)], MAP (λA. (-1, Pos (INR (Eqc A Y)))) As, 0)]
-    | INR cC => [
-        ([], MAP (λA. (1, Pos (INR (Eqc A Y)))) As, cC);
-        ([], MAP (λA. (-1, Pos (INR (Eqc A Y)))) As, -cC)]
-  in
-    encode_Gem_ge_iff bnd As Y ++
-    encode_Gem_le_iff bnd As Y ++
-    MAP (λA. bits_imply bnd [Pos (INR (Eqc A Y))]
-                        ([], [(1, Pos (INR (Gem A Y))); (1, Pos (INR (Gem Y A)))], 2)) As ++
-    MAP (λA. bits_imply bnd [Neg (INR (Eqc A Y))]
-                        ([], [(1, Neg (INR (Gem A Y))); (1, Neg (INR (Gem Y A)))], 1)) As ++
-    ilpc
-End
-
-Theorem encode_count_sem:
-  valid_assignment bnd wi ⇒
-  EVERY (λx. iconstraint_sem x (wi,wb)) (encode_count bnd Y C As) = (
-    EVERY (λA. wb (INR (Gem A Y)) ⇔ varc wi A ≥ varc wi Y) As ∧
-    EVERY (λA. wb (INR (Gem Y A)) ⇔ varc wi Y ≥ varc wi A) As ∧
-    EVERY (λA. wb (INR (Eqc A Y)) ⇔ varc wi A = varc wi Y) As ∧
-    count_sem Y C As wi)
-Proof
-  strip_tac>>
-  simp[encode_count_def]>>
-  simp[GSYM CONJ_ASSOC]>>
-  ho_match_mp_tac LEFT_AND_CONG>>
-  CONJ_TAC >-
-    simp[encode_Gem_ge_iff_sem,EVERY_MEM]>>
-  strip_tac>>
-  ho_match_mp_tac LEFT_AND_CONG>>
-  CONJ_TAC >-
-    simp[encode_Gem_le_iff_sem,EVERY_MEM,integerTheory.INT_GE]>>
-  strip_tac>>
-  simp[CONJ_ASSOC]>>
-  ho_match_mp_tac LEFT_AND_CONG>>
+  fs[enc_rel_def]>>
   CONJ_TAC >- (
-    fs[EVERY_MAP,EVERY_MEM,iconstraint_sem_def]>>
-    metis_tac[integerTheory.INT_LE_ANTISYM,integerTheory.INT_GE])>>
-  strip_tac
-  >- (
-    Cases_on ‘C’>>
-    simp[count_sem_def]>>
-    rw[METIS_PROVE[] “∀P a b. (∀x. x = a ∨ x = b ⇒ P x) ⇔ P a ∧ P b”]>>
-    simp[iconstraint_sem_def,eval_ilin_term_def,eval_lin_term_def,
-      MAP_MAP_o,combinTheory.o_ABS_R,b2i_alt,iSUM_def,Once varc_def]>>
-    ‘iSUM (MAP (λA. if wb (INR (Eqc A Y)) then 1 else 0) As) =
-     iSUM (MAP (λA. if varc wi A = varc wi Y then 1 else 0) As)’ by
-      fs[EVERY_MEM,Cong MAP_CONG]>>
-    simp[iSUM_MAP_lin_const]>>
-    intLib.ARITH_TAC)
+    fs[mods_fl_def]>>rw[]>>
+    first_x_assum drule>>rw[])>>
+  drule_all agree_on_fl_mods_fl_append>>
+  rw[]>>
+  metis_tac[]
 QED
 
 (***
-  NValue
+  Dealing with ge / eq
 ***)
-
-(* domain of X given by bnd (as a list) *)
-Definition domlist_def:
-  domlist bnd X =
-  let
-    (lb, ub) = bnd X
-  in
-    if ub < lb
-    then []
-    else GENLIST (λn. &n + lb) (Num (ub - lb) + 1)
+Definition add_ge_def:
+  add_ge Y n ec =
+  let tt =
+    (case ALOOKUP ec.ge Y of
+      NONE => []
+    | SOME ls => ls) in
+  ec with ge := (Y,n::tt)::ec.ge
 End
 
-Theorem MEM_domlist:
-  valid_assignment bnd wi ⇒
-  MEM (wi X) (domlist bnd X)
-Proof
-  Cases_on ‘bnd X’>>
-  rw[domlist_def,valid_assignment_def,MEM_GENLIST]>>
-  res_tac
-  >-(
-    goal_assum $ drule_at Any>>
-    intLib.ARITH_TAC)>>
-  intLib.ARITH_TAC
-QED
-
-(* bijection 0, -1, 1, -2, 2,... ⇔ 0, 1, 2, 3, 4,... and its inverse next *)
-Definition intnum_def:
-  intnum (n: int) =
-  if n < 0 then 2 * Num (-n) - 1
-  else 2 * Num n
+Definition add_eq_def:
+  add_eq Y n ec =
+  let tt =
+    (case ALOOKUP ec.eq Y of
+      NONE => []
+    | SOME ls => ls) in
+  ec with eq := (Y,n::tt)::ec.eq
 End
 
-Definition numint_def:
-  numint (n: num): int =
-  if EVEN n then &((n + 1) DIV 2)
-  else -&((n + 1) DIV 2)
+Theorem add_ge_fresh[simp]:
+  (add_ge Y n ec).fresh = ec.fresh
+Proof
+  rw[add_ge_def]
+QED
+
+Theorem add_eq_fresh[simp]:
+  (add_eq Y n ec).fresh = ec.fresh
+Proof
+  rw[add_eq_def]
+QED
+
+Theorem has_ge_add_ge[simp]:
+  has_ge X n (add_ge Y m ec) ⇔
+  X = Y ∧ n = m ∨
+  has_ge X n ec
+Proof
+  rw[has_ge_def,add_ge_def]>>every_case_tac>>simp[]
+QED
+
+Theorem has_ge_add_eq[simp]:
+  has_ge X n (add_eq Y m ec) ⇔
+  has_ge X n ec
+Proof
+  rw[has_ge_def,add_eq_def]>>every_case_tac>>simp[]
+QED
+
+Theorem has_eq_add_eq[simp]:
+  has_eq X n (add_eq Y m ec) ⇔
+  X = Y ∧ n = m ∨
+  has_eq X n ec
+Proof
+  rw[has_eq_def,add_eq_def]>>every_case_tac>>simp[]
+QED
+
+Theorem has_eq_add_ge[simp]:
+  has_eq X n (add_ge Y m ec) ⇔
+  has_eq X n ec
+Proof
+  rw[has_eq_def,add_ge_def]>>every_case_tac>>simp[]
+QED
+
+(* TODO: what annotation should we use? *)
+Definition cencode_ge_def:
+  cencode_ge bnd Y n ec =
+  if has_ge Y n ec
+  then (Nil, ec)
+  else
+    let ec = add_ge Y n ec in
+    (List (MAP (\x. (NONE,x)) (encode_ge bnd Y n)), ec)
 End
 
-Theorem numint_inj:
-  numint m = numint n ⇒ m = n
-Proof
-  simp[numint_def]>>
-  intLib.ARITH_TAC
-QED
-
-Theorem numint_intnum:
-  numint (intnum x) = x
-Proof
-  simp[intnum_def,numint_def]>>
-  intLib.ARITH_TAC
-QED
-
-Theorem intnum_numint:
-  intnum (numint x) = x
-Proof
-  simp[intnum_def,numint_def]>>
-  intLib.ARITH_TAC
-QED
-
-Definition numset_to_intlist_def:
-  numset_to_intlist t = MAP (numint o FST) $ toSortedAList t
-End
-
-Theorem ALL_DISTINCT_numset_to_intlist:
-  ALL_DISTINCT $ numset_to_intlist t
-Proof
-  simp[numset_to_intlist_def,GSYM MAP_MAP_o]>>
-  irule ALL_DISTINCT_MAP_INJ>>
-  simp[ALL_DISTINCT_MAP_FST_toSortedAList,numint_inj]
-QED
-
-(* Union of all int values in domains of Xs *)
-Definition union_dom_def:
-  union_dom bnd Xs =
-  numset_to_intlist $ FOLDL union LN $
-    MAP (λX. list_to_num_set $ MAP intnum $ domlist bnd X) Xs
-End
-
-Theorem MEM_numset_to_intlist:
-  MEM x (numset_to_intlist ns) ⇔
-  intnum x ∈ domain ns
-Proof
-  rw[numset_to_intlist_def,GSYM MAP_MAP_o,MEM_MAP,EXISTS_PROD,
-    MEM_toSortedAList,domain_lookup]>>
-  metis_tac[intnum_numint,numint_intnum]
-QED
-
-Theorem domain_FOLDL_union:
-  ∀ls t.
-  x ∈ domain (FOLDL union t ls) ⇔
-  x ∈ domain t ∨ ∃ns. ns ∈ set ls ∧ x ∈ domain ns
-Proof
-  Induct>>rw[]>>
-  metis_tac[]
-QED
-
-Theorem EVERY_MEM_union_dom:
-  valid_assignment bnd wi ⇒
-  EVERY (λA. MEM (wi A) (union_dom bnd Xs)) Xs
-Proof
-  rw[EVERY_MEM,union_dom_def,MEM_numset_to_intlist,domain_FOLDL_union]>>
-  simp[MEM_MAP,PULL_EXISTS,domain_list_to_num_set]>>
-  metis_tac[MEM_domlist]
-QED
-
-Theorem ALL_DISTINCT_union_dom:
-  ALL_DISTINCT $ union_dom bnd Xs
-Proof
-  simp[union_dom_def,ALL_DISTINCT_numset_to_intlist]
-QED
-
-(* encodes fnvalue_v ⇔ some X = v *)
-Definition encode_some_eq_def:
-  encode_some_eq bnd Xs (v: int) =
-    bimply_bits bnd [Pos (INR (Nv Xs v))]
-      ([], MAP (λA. (1i, Pos (INL (Eq A v)))) Xs, 1i)
-End
-
-Theorem encode_some_eq_sem:
-  valid_assignment bnd wi ∧
-  EVERY (λX. wb (INL (Eq X v)) ⇔ wi X = v) Xs ⇒
-  (EVERY (λx. iconstraint_sem x (wi,wb)) (encode_some_eq bnd Xs v) =
-  (wb (INR (Nv Xs v)) ⇔ ∃A. MEM A Xs ∧ wb (INL (Eq A v))))
-Proof
-  rw[encode_some_eq_def,iconstraint_sem_def,eval_lin_term_ge_1]>>
-  metis_tac[]
-QED
-
-Definition reify_some_eq_def:
-  reify_some_eq bnd Xs v =
-  let
-    ges = FLAT $ MAP (λX. encode_ge bnd X v ++ encode_ge bnd X (v + 1)) Xs;
-    eqs = FLAT $ MAP (λX. encode_eq bnd X v) Xs
-  in
-    ges ++ eqs ++ encode_some_eq bnd Xs v
-End
-
-Theorem reify_some_eq_sem:
-  valid_assignment bnd wi ⇒ (
-  EVERY (λx. iconstraint_sem x (wi,wb)) (FLAT (MAP (reify_some_eq bnd Xs)
-    (union_dom bnd Xs))) ⇔
-  ∀v. MEM v (union_dom bnd Xs) ⇒
-      EVERY (λX. wb (INL (Ge X v)) ⇔ wi X ≥ v) Xs ∧
-      EVERY (λX. wb (INL (Ge X (v + 1))) ⇔ wi X ≥ v + 1) Xs ∧
-      EVERY (λX. wb (INL (Eq X v)) ⇔ wi X = v) Xs ∧
-      (wb (INR (Nv Xs v)) ⇔ ∃A. MEM A Xs ∧ wb (INL (Eq A v))))
-Proof
-  rw[reify_some_eq_def,EVERY_FLAT,EVERY_MAP]>>
-  simp[Once EVERY_MEM,Once $ GSYM CONJ_ASSOC]>>
-  ho_match_mp_tac FORALL_IMP_EQ>>
-  rw[EVERY_CONJ,GSYM CONJ_ASSOC]>>
-  match_mp_tac LEFT_AND_CONG>>
-  CONJ_TAC
-  >- (irule EVERY_CONG>>simp[encode_ge_sem])>>
-  strip_tac>>
-  match_mp_tac LEFT_AND_CONG>>
-  CONJ_TAC
-  >- (irule EVERY_CONG>>simp[encode_ge_sem])>>
-  strip_tac>>
-  match_mp_tac LEFT_AND_CONG>>
-  CONJ_TAC
-  >- (
-    irule EVERY_CONG>>
-    rw[]>>
-    irule encode_eq_sem>>
-    fs[EVERY_MEM])>>
-  simp[encode_some_eq_sem]
-QED
-
-(* encodes (sum of the bitlist Bs) = Y *)
-Definition encode_bitsum_def:
-  encode_bitsum Bs Y =
-  case Y of
-    INL vY => [
-      ([(-1i, vY)], MAP (λb. (1i, Pos b)) Bs, 0i);
-      ([(1i, vY)], MAP (λb. (-1i, Pos b)) Bs, 0i)]
-  | INR cY => [
-      ([], MAP (λb. (1i, Pos b)) Bs, cY);
-      ([], MAP (λb. (-1i, Pos b)) Bs, -cY)]
-End
-
-Theorem encode_bitsum_sem:
-  valid_assignment bnd wi ⇒
-  (EVERY (λx. iconstraint_sem x (wi,wb)) (encode_bitsum Bs Y) ⇔
-  iSUM $ MAP (b2i o wb) Bs = varc wi Y)
-Proof
-  rw[encode_bitsum_def]>>
-  CASE_TAC>>
-  simp[varc_def,iconstraint_sem_def,eval_ilin_term_def,eval_lin_term_def,
-    eval_iterm_def,eval_term_def,iSUM_def,MAP_MAP_o,combinTheory.o_ABS_R,
-    iSUM_MAP_lin_const]>>
-  simp[GSYM combinTheory.o_ABS_R,GSYM combinTheory.I_EQ_IDABS]>>
-  intLib.ARITH_TAC
-QED
-
-Theorem encode_nvalue_sem_aux:
-  valid_assignment bnd wi ∧
-  (∀v. MEM v (union_dom bnd Xs) ⇒
-    EVERY (λX. wb (INL (Eq X v)) ⇔ wi X = v) Xs ∧
-    (wb (INR (Nv Xs v)) ⇔ ∃A. MEM A Xs ∧ wb (INL (Eq A v)))) ⇒
-  ∀v. MEM v (MAP wi Xs) ⇔ MEM v (FILTER (λv. wb (INR (Nv Xs v))) (union_dom bnd Xs))
-Proof
-  rw[MEM_FILTER,MEM_MAP]>>
-  iff_tac>>
-  strip_tac
-  >-(
-    CONJ_ASM2_TAC
-    >- (
-      gvs[EVERY_MEM]>>
-      metis_tac[])>>
-    drule_then assume_tac EVERY_MEM_union_dom>>
-    fs[EVERY_MEM])>>
-  gvs[EVERY_MEM]>>
-  metis_tac[]
-QED
-
-Theorem list_set_eq:
-  ∀ls1 ls2. (∀v. MEM v ls1 ⇔ MEM v ls2) ⇔ set ls1 = set ls2
-Proof
-  rw[SET_EQ_SUBSET]>>
-  simp[GSYM SUBSET_DIFF_EMPTY,list_to_set_diff,GSYM NULL_EQ,NULL_FILTER]>>
-  metis_tac[]
-QED
-
+(* TODO: lemmas *)
 Theorem iSUM_FILTER:
   iSUM (MAP (b2i o P) ls) = &(LENGTH $ FILTER P ls)
 Proof
@@ -1328,338 +413,59 @@ Proof
   intLib.ARITH_TAC
 QED
 
-Definition encode_nvalue_def:
-  encode_nvalue bnd Y Xs =
-  let
-    vals = union_dom bnd Xs;
-  in
-    (FLAT $ MAP (reify_some_eq bnd Xs) vals) ++
-    encode_bitsum (MAP (λv. INR (Nv Xs v)) vals) Y
-End
-
-Theorem encode_nvalue_sem:
-  valid_assignment bnd wi ⇒
-  EVERY (λx. iconstraint_sem x (wi,wb)) (encode_nvalue bnd Y Xs) = (
-    nvalue_sem Y Xs wi ∧
-    ∀v. MEM v (union_dom bnd Xs) ⇒
-        EVERY (λX. wb (INL (Ge X v)) ⇔ wi X ≥ v) Xs ∧
-        EVERY (λX. wb (INL (Ge X (v + 1))) ⇔ wi X ≥ v + 1) Xs ∧
-        EVERY (λX. wb (INL (Eq X v)) ⇔ wi X = v) Xs ∧
-        (wb (INR (Nv Xs v)) ⇔ ∃A. MEM A Xs ∧ wb (INL (Eq A v))))
+Theorem iSUM_MAP_b2i_bound:
+  0 ≤ iSUM (MAP (λp. b2i (f p)) ls) ∧
+  iSUM (MAP (λp. b2i (f p)) ls) ≤ &LENGTH ls
 Proof
-  rw[encode_nvalue_def,Once CONJ_COMM]>>
-  match_mp_tac $ METIS_PROVE[] “(Q ⇔ Q') ∧ (Q' ⇒ (P ⇔ P')) ⇒ (P ∧ Q ⇔ P' ∧ Q')”>>
-  CONJ_TAC>>
-  simp[reify_some_eq_sem]>>
-  strip_tac>>
-  ‘∀v. MEM v (union_dom bnd Xs) ⇒
-    EVERY (λX. wb (INL (Eq X v)) ⇔ wi X = v) Xs ∧
-    (wb (INR (Nv Xs v)) ⇔ ∃A. MEM A Xs ∧ wb (INL (Eq A v)))’ by metis_tac[]>>
-  drule_all_then assume_tac encode_nvalue_sem_aux>>
-  DEP_REWRITE_TAC[encode_bitsum_sem]>>
-  gs[nvalue_sem_def,iSUM_FILTER,FILTER_MAP,o_DEF,list_set_eq,
-     ALL_DISTINCT_union_dom,FILTER_ALL_DISTINCT,ALL_DISTINCT_CARD_LIST_TO_SET]>>
+  Induct_on`ls`>>rw[iSUM_def,oneline b2i_def]>>
   intLib.ARITH_TAC
 QED
 
-(***
-  Table
-***)
-
-(* encodes ftable_i ⇔ X = Ti, provided that LENGTH X = LENGTH Ti *)
-Definition encode_tuple_eq_def:
-  encode_tuple_eq bnd Xs Ys =
-    bimply_bits bnd [Pos (INR (Tb Xs Ys))]
-      ([], MAP2 (λX Y. (1i, Pos (INL (Eq X Y)))) Xs Ys, &LENGTH Xs)
-End
-
-Definition reify_tuple_eq_def:
-  reify_tuple_eq bnd Xs Ys =
-  let
-    ges = FLAT $ MAP2 (λX Y. encode_ge bnd X Y ++ encode_ge bnd X (Y + 1)) Xs Ys;
-    eqs = FLAT $ MAP2 (λX Y. encode_eq bnd X Y) Xs Ys
-  in
-    ges ++ eqs ++ encode_tuple_eq bnd Xs Ys
-End
-
-Theorem LENGTH_FILTER_LE:
-  LENGTH ls ≤ LENGTH (FILTER P ls) ⇔ LENGTH ls = LENGTH (FILTER P ls)
+Theorem add_ge_flip[local]:
+  (a + x ≥ y ⇔
+  y - (a:int) ≤ x)
 Proof
-  metis_tac[GREATER_EQ,LE_ANTISYM,LENGTH_FILTER_LEQ]
+  intLib.ARITH_TAC
 QED
 
-Theorem LENGTH_FILTER_EQ:
-  LENGTH ls = LENGTH (FILTER P ls) ⇔ EVERY P ls
+Theorem iSUM_MAP_b2i_ge_1[simp]:
+  ∀ls.
+  iSUM (MAP (λp. b2i (f p)) ls) ≥ 1 ⇔
+  ∃x. MEM x ls ∧ f x
 Proof
-  Induct_on ‘ls’>>
-  rw[FILTER,ADD1]>>
-  irule $ intLib.ARITH_PROVE “(a:num) > b ⇒ a ≠ b”>>
-  simp[GREATER_DEF,GSYM LE_LT1,LENGTH_FILTER_LEQ,LENGTH_FILTER_LEQ]
-QED
-
-Theorem reify_tuple_eq_aux[local]:
-  valid_assignment bnd wi ⇒ (
-  LIST_REL (λX Y.
-    (wb (INL (Ge X Y)) ⇔ wi X ≥ Y) ∧
-    (wb (INL (Ge X (Y + 1))) ⇔ wi X ≥ Y + 1) ∧
-    EVERY (λx. iconstraint_sem x (wi,wb)) (encode_eq bnd X Y)) Xs Ys ⇔
-  LIST_REL (λX Y.
-    (wb (INL (Ge X Y)) ⇔ wi X ≥ Y) ∧
-    (wb (INL (Ge X (Y + 1))) ⇔ wi X ≥ Y + 1) ∧
-    (wb (INL (Eq X Y)) ⇔ wi X = Y)) Xs Ys)
-Proof
-  strip_tac>>
-  simp[LIST_REL_EVERY_ZIP,Once EVERY_MEM,Once EQ_SYM_EQ]>>
-  simp[Once EVERY_MEM]>>
-  ho_match_mp_tac $ METIS_PROVE[]
-    “(∀x. Q x ⇒ (R1 x ⇔ R2 x)) ⇒ ((P ∧ ∀x. Q x ⇒ R1 x) ⇔ (P ∧ ∀x. Q x ⇒ R2 x))”>>
-  rw[]>>
-  pairarg_tac>>
-  simp[BETA_THM]>>
-  METIS_TAC[encode_eq_sem]
-QED
-
-Theorem encode_tuple_eq_sem:
-  valid_assignment bnd wi ∧
-  LENGTH Xs = LENGTH Ys ∧
-  LIST_REL (λX Y. wb (INL (Eq X Y)) ⇔ wi X = Y) Xs Ys
-  ⇒
-  (EVERY (λx. iconstraint_sem x (wi,wb))
-    (encode_tuple_eq bnd Xs Ys) ⇔
-  (wb (INR (Tb Xs Ys)) ⇔ LIST_REL (λX Y. wi X = Y) Xs Ys))
-Proof
-  rw[encode_tuple_eq_def,iconstraint_sem_def]>>
-  simp[MAP2_ZIP,EQ_SYM_EQ,eval_lin_term_def,
-    MAP_MAP_o,iterateTheory.LAMBDA_PAIR,
-    combinTheory.o_ABS_R,iSUM_FILTER]>>
-  qho_match_abbrev_tac ‘((R ⇔ P) ⇔ (R ⇔ Q))’>>
-  qsuff_tac ‘P ⇔ Q’
-  >-metis_tac[]>>
-  unabbrev_all_tac>>
-  fs[Once $ GSYM combinTheory.o_ABS_R,iSUM_FILTER,LIST_REL_EVERY_ZIP]>>
-  drule_then assume_tac $ cj 2 LENGTH_ZIP>>
-  pop_assum (SUBST_ALL_TAC o SYM)>>
-  pure_rewrite_tac[intReduceTheory.INT_GE_CONV_pth,
-    LENGTH_FILTER_LE,LENGTH_FILTER_EQ]>>
-  fs[EVERY_MEM]>>
-  ho_match_mp_tac FORALL_IMP_EQ>>
-  fs[EQ_SYM_EQ,iterateTheory.LAMBDA_PAIR]
-QED
-
-Theorem reify_tuple_eq_sem:
-  valid_assignment bnd wi ∧
-  LENGTH Xs = LENGTH Ys ⇒ (
-  EVERY (λx. iconstraint_sem x (wi,wb))
-    (reify_tuple_eq bnd Xs Ys) ⇔
-    LIST_REL (λX Y.
-      (wb (INL (Ge X Y)) ⇔ wi X ≥ Y) ∧
-      (wb (INL (Ge X (Y + 1))) ⇔ wi X ≥ Y + 1) ∧
-      (wb (INL (Eq X Y)) ⇔ wi X = Y)) Xs Ys ∧
-    (wb (INR (Tb Xs Ys)) ⇔
-      LIST_REL (λX Y. wi X = Y) Xs Ys))
-Proof
-  simp[LIST_REL_CONJ]>>
-  rw[reify_tuple_eq_def,EVERY_FLAT]>>
-  simp[GSYM CONJ_ASSOC]>>
-  simp[Once CONJ_ASSOC, SimpRHS]>>
-  ho_match_mp_tac LEFT_AND_CONG >> simp[]>>
-  CONJ_TAC
+  Induct_on`ls`>>
+  rw[iSUM_def]>>
+  rw[Once (oneline b2i_def)]
   >- (
-    simp[Once EVERY_MEM]>>
-    simp[LIST_REL_EVERY_ZIP,EVERY_MEM,SimpRHS]>>
-    simp[MAP2_ZIP,MEM_MAP,PULL_EXISTS,MEM_ZIP]>>
+    simp[add_ge_flip]>>
+    metis_tac[iSUM_MAP_b2i_bound])>>
+  metis_tac[]
+QED
+
+Theorem iSUM_MAP_b2i_ge_LENGTH[simp]:
+  ∀ls.
+  iSUM (MAP (λp. b2i (f p)) ls) ≥ &LENGTH ls ⇔
+  (∀x. MEM x ls ⇒ f x)
+Proof
+  Induct_on`ls`>>
+  rw[iSUM_def]>>
+  rw[Once (oneline b2i_def)]
+  >- (
+    fs[add_ge_flip,ADD1,integerTheory.int_ge]>>
+    simp[GSYM integerTheory.INT_ADD,int_arithTheory.elim_minus_ones]>>
     metis_tac[])>>
-  strip_tac>>
-  ho_match_mp_tac LEFT_AND_CONG >> simp[]>>
-  CONJ_TAC
-  >- (
-    simp[Once EVERY_MEM]>>
-    simp[LIST_REL_EVERY_ZIP,EVERY_MEM,SimpRHS]>>
-    simp[MAP2_ZIP,MEM_MAP,PULL_EXISTS,MEM_ZIP]>>
-    ho_match_mp_tac FORALL_IMP_EQ>>
-    rw[]>>
-    DEP_REWRITE_TAC[encode_eq_sem]>>simp[]>>
-    gvs[LIST_REL_EL_EQN])>>
-  strip_tac>>
-  metis_tac[encode_tuple_eq_sem]
+  assume_tac iSUM_MAP_b2i_bound>>
+  simp[SF DNF_ss]>>
+  intLib.ARITH_TAC
 QED
 
-Definition encode_table_def:
-  encode_table bnd Xs Yss =
-  let n = LENGTH Xs in
-    if EVERY (λYs. LENGTH Ys = n) Yss
-    then
-      (FLAT $ MAP (λYs. reify_tuple_eq bnd Xs Ys) Yss) ++
-      [([], MAP (λYs. (1i, Pos (INR (Tb Xs Ys)))) Yss, 1)]
-    else
-      [([], [], 1i)]
+Definition false_constr_def:
+  false_constr = ([], [], 1i)
 End
 
-Theorem MAP_LIST_REL:
-  MAP f Xs = Ys ⇔ LIST_REL (λx y. f x = y) Xs Ys
+Theorem iconstraint_sem_false_constr[simp]:
+  ¬iconstraint_sem false_constr w
 Proof
-  ‘MAP f Xs = MAP I Ys ⇔ LIST_REL (λx y. f x = I y) Xs Ys’ suffices_by simp[MAP_ID]>>
-  metis_tac[MAP_EQ_EVERY2,EVERY2_LENGTH]
+  Cases_on`w`>>EVAL_TAC
 QED
 
-(* assume that Xs are all variables *)
-Theorem encode_table_sem:
-  valid_assignment bnd wi ⇒
-  EVERY (λx. iconstraint_sem x (wi,wb)) (encode_table bnd Xs Yss) = (
-    table_sem Xs Yss wi ∧
-    (∀Ys. MEM Ys Yss ⇒
-      LIST_REL (λX Y.
-        (wb (INL (Ge X Y)) ⇔ wi X ≥ Y) ∧
-        (wb (INL (Ge X (Y + 1))) ⇔ wi X ≥ Y + 1) ∧
-        (wb (INL (Eq X Y)) ⇔ wi X = Y)) Xs Ys ∧
-      (wb (INR (Tb Xs Ys)) ⇔
-        LIST_REL (λX Y. wi X = Y) Xs Ys)) ∧
-    (∃Ys. MEM Ys Yss ∧ wb (INR (Tb Xs Ys))))
-Proof
-  rw[encode_table_def,table_sem_def,iconstraint_sem_def,
-    eval_ilin_term_def,eval_lin_term_def,iSUM_def]>>
-  last_x_assum $ mp_tac>>
-  simp[Once EVERY_MEM,EVERY_FLAT,EVERY_MAP,Once EVERY_MEM,MAP_MAP_o,
-    combinTheory.o_ABS_R]>>
-  rw[Once $ GSYM combinTheory.o_ABS_R,iSUM_FILTER,Once integerTheory.INT_GE,
-    intLib.ARITH_PROVE “1i ≤ m ⇔ 0i < m”,LENGTH_NOT_NULL,NULL_FILTER]>>
-  ho_match_mp_tac (METIS_PROVE[]
-    “(∀x. P1 x ⇒ (Q1 x ⇔ Q2 x)) ∧
-    ((∀x. P1 x ⇒ Q2 x) ∧ R ⇒ P2) ⇒
-    ((∀x. P1 x ⇒ Q1 x) ∧ R ⇔ (P2 ∧ (∀x. P1 x ⇒ Q2 x) ∧ R))”)>>
-  CONJ_TAC>>
-  rw[]>>
-  gvs[reify_tuple_eq_sem,GSYM MAP_LIST_REL]
-QED
-
-(* The top-level encodings *)
-Definition encode_cp_one_def:
-  encode_cp_one bnd c =
-  case c of
-    NotEquals X Y => encode_not_equals bnd X Y
-  | AllDifferent As => encode_all_different bnd As
-  | Element R X As => encode_element bnd R X As
-  | Element2D R X Y Tss => encode_element2d bnd R X Y Tss
-  | Abs X Y => encode_abs bnd X Y
-  | Ilc Xs op rhs => encode_ilc Xs op rhs
-  | ArrMax M As => encode_arr_max bnd M As
-  | ArrMin M As => encode_arr_min bnd M As
-  | Count Y C As => encode_count bnd Y C As
-  | Nvalue Y Xs => encode_nvalue bnd Y Xs
-  | Table Xs Yss => encode_table bnd Xs Yss
-End
-
-Theorem encode_cp_one_sem_1:
-  valid_assignment bnd wi ∧
-  constraint_sem c wi ⇒
-  EVERY (λx. iconstraint_sem x (wi,reify_avar wi)) (encode_cp_one bnd c)
-Proof
-  Cases_on`c`>>
-  rw[encode_cp_one_def,constraint_sem_def]
-  >- (
-    simp[encode_not_equals_sem,reify_avar_def,reify_flag_def]>>
-    gvs[not_equals_sem_def]>>
-    intLib.ARITH_TAC)
-  >- (
-    simp[encode_all_different_sem,reify_avar_def,reify_flag_def]>>
-    gvs[all_different_sem_def,EL_ALL_DISTINCT_EL_EQ]>>
-    rw[]>>
-    first_x_assum(qspecl_then[`i`,`j`] mp_tac)>>
-    simp[EL_MAP]>>
-    intLib.ARITH_TAC)
-  >- (
-    simp[encode_element_sem,reify_avar_def,reify_flag_def,reify_reif_def]>>
-    every_case_tac>>simp[])
-  >- (
-    simp[encode_element2d_sem,reify_avar_def,reify_reif_def]>>
-    every_case_tac)
-  >- (
-    simp[encode_abs_sem,reify_avar_def,reify_reif_def]>>
-    every_case_tac>>simp[])
-  >- (
-    simp[encode_ilc_sem,reify_avar_def]>>
-    every_case_tac>>simp[])
-  >- (
-    fs[encode_arr_max_sem,reify_avar_def,reify_flag_def,arr_max_sem_def]>>
-    fs[MEM_MAP]>>
-    goal_assum $ drule_at Any>>
-    simp[integerTheory.int_ge,integerTheory.INT_LE_REFL])
-  >- (
-    fs[encode_arr_min_sem,reify_avar_def,reify_flag_def,arr_min_sem_def]>>
-    fs[MEM_MAP,integerTheory.int_ge]>>
-    goal_assum $ drule_at Any>>
-    simp[integerTheory.int_ge,integerTheory.INT_LE_REFL])
-  >-simp[encode_count_sem,reify_avar_def,reify_flag_def]
-  >- (
-    fs[encode_nvalue_sem,reify_avar_def,nvalue_sem_def,MEM_MAP,reify_reif_def,reify_flag_def]>>
-    metis_tac[])
-  >- (
-    fs[encode_table_sem,reify_avar_def,table_sem_def,reify_reif_def,reify_flag_def]>>
-    rw[LIST_REL_EL_EQN,EVERY_MEM]>>
-    fs[MAP_LIST_REL,EVERY_MEM,LIST_REL_EL_EQN])
-QED
-
-Theorem encode_cp_one_sem_2:
-  valid_assignment bnd wi ∧
-  EVERY (λx. iconstraint_sem x (wi,wb)) (encode_cp_one bnd c) ⇒
-  constraint_sem c wi
-Proof
-  Cases_on`c`>>
-  rw[encode_cp_one_def,constraint_sem_def]
-  >-gvs[encode_not_equals_sem]
-  >-gvs[encode_all_different_sem]
-  >-gvs[encode_element_sem]
-  >-gvs[encode_element2d_sem]
-  >-gvs[encode_abs_sem]
-  >-gvs[encode_ilc_sem]
-  >-gvs[encode_arr_max_sem]
-  >-gvs[encode_arr_min_sem]
-  >-gvs[encode_count_sem]
-  >-gvs[encode_nvalue_sem]
-  >-gvs[encode_table_sem]
-QED
-
-(* An actual implementation will avoid duplicates here *)
-Definition encode_cp_all_def:
-  encode_cp_all bnd cs =
-  FLAT (MAP (encode_cp_one bnd) cs)
-End
-
-Theorem encode_cp_all_sem_1:
-  valid_assignment bnd wi ∧
-  EVERY (λc. constraint_sem c wi) cs ⇒
-  EVERY (λx. iconstraint_sem x (wi,reify_avar wi)) (encode_cp_all bnd cs)
-Proof
-  simp[encode_cp_all_def,EVERY_FLAT]>>
-  simp[Once EVERY_MEM]>>
-  rw[Once EVERY_MEM,MEM_MAP]>>
-  metis_tac[encode_cp_one_sem_1]
-QED
-
-Theorem encode_cp_all_sem_2:
-  valid_assignment bnd wi ∧
-  EVERY (λx. iconstraint_sem x (wi,wb)) (encode_cp_all bnd cs) ⇒
-  EVERY (λc. constraint_sem c wi) cs
-Proof
-  simp[encode_cp_all_def,EVERY_FLAT]>>
-  rw[Once EVERY_MEM,MEM_MAP,PULL_EXISTS]>>
-  simp[Once EVERY_MEM]>>
-  metis_tac[encode_cp_one_sem_2]
-QED
-
-(* === Examples ===
-
-not-equals
-  EVAL``encode_not_equals (λX. (-10,10)) (INL X) (INL Y)``
-  EVAL``encode_not_equals (λX. (-10,10)) (INL X) (INR 4)``
-
-all-different
-  EVAL``encode_all_different (λX. (-10,10)) [INL X; INL Y; INL Z; INR 0i]``
-
-element
-  EVAL``encode_element (λX. (-10,10)) (INL R) (INL X) [INL A; INL B; INL C; INL D; INL E]``
-
-abs
-  EVAL``encode_abs (λX. (-10,10)) (INL X) (INL Y)``
-
-*)
