examples/pseudo_bool/cp_encoding/cp_to_ilp_extensionalScript.sml
@@ -1,0 +1,216 @@
+(*
+  Formalization of the CP to ILP phase (extensional constraints)
+*)
+Theory cp_to_ilp_extensional
+Libs
+  preamble
+Ancestors
+  pbc cp ilp cp_to_ilp
+
+(* Keep only the positions that we need to match *)
+Definition filter_match_def:
+  (filter_match [] = []) ∧
+  (filter_match ((x,topt)::xs) =
+    case topt of
+      NONE => filter_match xs
+    | SOME t => (x,t)::filter_match xs)
+End
+
+(* encodes ftable_i ⇔ X = Ti, provided that LENGTH X = LENGTH Ti *)
+Definition encode_tuple_eq_def:
+  encode_tuple_eq bnd Xts =
+    bimply_bits bnd [Pos (INR (Tb Xts))]
+      ([], MAP (λ(X,t). (1i, Pos (INL (Eq X t)))) Xts, &LENGTH Xts)
+End
+
+(* The reifications needed for tuple eq on a given row *)
+Definition reify_tuple_eq_def:
+  reify_tuple_eq bnd Xts =
+  let
+    ges = FLAT $ MAP (λ(X,t). encode_ge bnd X t ++ encode_ge bnd X (t + 1)) Xts;
+    eqs = FLAT $ MAP (λ(X,t). encode_eq bnd X t) Xts
+  in
+    ges ++ eqs ++ encode_tuple_eq bnd Xts
+End
+
+Theorem encode_tuple_eq_sem:
+  valid_assignment bnd wi ∧
+  EVERY (λ(X,t). wb (INL (Eq X t)) ⇔ wi X = t) Xts
+  ⇒
+  (EVERY (λx. iconstraint_sem x (wi,wb))
+    (encode_tuple_eq bnd Xts) ⇔
+  (wb (INR (Tb Xts)) ⇔ EVERY (λ(X,t). wi X = t) Xts))
+Proof
+  rw[encode_tuple_eq_def,iconstraint_sem_def]>>
+  simp[eval_lin_term_def]>>
+  qho_match_abbrev_tac ‘((P ⇔ R) ⇔ (R ⇔ Q))’>>
+  qsuff_tac ‘P ⇔ Q’
+  >-metis_tac[]>>
+  unabbrev_all_tac>>
+  pop_assum mp_tac>>
+  last_x_assum kall_tac>>
+  Induct_on`Xts`>>rw[iSUM_def]>>
+  pairarg_tac>>gvs[]>>
+  rw[oneline b2i_def]>>gvs[]
+  >- (
+    last_x_assum sym_sub_tac>>
+    intLib.ARITH_TAC) >>
+  simp[MAP_MAP_o,o_DEF,iterateTheory.LAMBDA_PAIR]>>
+  qho_match_abbrev_tac`¬ (iSUM (MAP (λx. b2i (f x)) ls) ≥ _)`>>
+  `iSUM (MAP (λx. b2i (f x)) ls) ≤ &LENGTH ls` by
+    metis_tac[iSUM_MAP_b2i_bound]>>
+  intLib.ARITH_TAC
+QED
+
+Definition encode_table_def:
+  encode_table bnd tss Xs =
+  let n = LENGTH Xs in
+    if EVERY (λYs. LENGTH Ys = n) tss
+    then
+      let Xtss = MAP (λts. filter_match (ZIP (Xs,ts))) tss in
+      (FLAT $ MAP (λXts. reify_tuple_eq bnd Xts) Xtss) ++
+      [([], MAP (λXts. (1i, Pos (INR (Tb Xts)))) Xtss, 1)]
+    else
+      [false_constr]
+End
+
+Theorem match_row_filter_match:
+  ∀Xs ts.
+  LENGTH ts = LENGTH Xs ⇒
+  (match_row ts (MAP wi Xs) ⇔
+  EVERY (λ(X,t). wi X = t) (filter_match (ZIP (Xs,ts))))
+Proof
+  Induct>>rw[]>>
+  fs[filter_match_def,match_row_def,LENGTH_CONS]>>
+  TOP_CASE_TAC>>gvs[]>>
+  metis_tac[]
+QED
+
+Theorem encode_tuple_eq_sem_reify:
+  valid_assignment bnd wi  ⇒
+  EVERY (λx. iconstraint_sem x (wi,reify_avar wi)) (encode_tuple_eq bnd Xts)
+Proof
+  rw[encode_tuple_eq_def,reify_avar_def,reify_flag_def]>>
+  simp[iconstraint_sem_def,MAP_MAP_o,o_DEF,eval_lin_term_def,iterateTheory.LAMBDA_PAIR,
+    reify_avar_def,reify_reif_def,EVERY_MEM]
+QED
+
+Theorem reify_tuple_eq_sem_reify:
+  valid_assignment bnd wi  ⇒
+  EVERY (λx. iconstraint_sem x (wi,reify_avar wi)) (reify_tuple_eq bnd Xts)
+Proof
+  rw[reify_tuple_eq_def]>>
+  simp[EVERY_FLAT]
+  >- simp[Once EVERY_MEM,MEM_MAP,PULL_EXISTS,FORALL_PROD,reify_avar_def,reify_reif_def]
+  >- simp[Once EVERY_MEM,MEM_MAP,PULL_EXISTS,FORALL_PROD,reify_avar_def,reify_reif_def]>>
+  metis_tac[encode_tuple_eq_sem_reify]
+QED
+
+Theorem encode_table_sem_1:
+  valid_assignment bnd wi ∧
+  table_sem tss Xs wi ⇒
+  EVERY (λx. iconstraint_sem x (wi,reify_avar wi)) (encode_table bnd tss Xs)
+Proof
+  simp[encode_table_def,table_sem_def]>>
+  strip_tac>>
+  CONJ_TAC >-
+    simp[EVERY_FLAT,EVERY_MAP,EVERY_FLAT,Once EVERY_MEM,reify_tuple_eq_sem_reify]>>
+  fs[EVERY_MEM]>>first_x_assum drule>>
+  strip_tac>> gs[match_row_filter_match]>>
+  simp[iconstraint_sem_def,MAP_MAP_o,o_DEF,eval_lin_term_def,reify_avar_def,reify_flag_def]>>
+  metis_tac[]
+QED
+
+Theorem reify_tuple_eq_sem:
+  valid_assignment bnd wi ∧
+  wb (INR (Tb Xts)) ∧
+  EVERY (λx. iconstraint_sem x (wi,wb))
+    (reify_tuple_eq bnd Xts) ⇒
+  EVERY (λ(X,t). wi X = t) Xts
+Proof
+  rw[reify_tuple_eq_def]>>
+  pop_assum mp_tac>>
+  DEP_REWRITE_TAC[encode_tuple_eq_sem]>>
+  rw[EVERY_MEM]>>
+  qpat_x_assum`EVERY _ (FLAT _)` mp_tac>>
+  simp[EVERY_FLAT,MAP_MAP_o,o_DEF,EVERY_MAP]>>
+  simp[Once EVERY_MEM]>>
+  disch_then drule>>
+  pairarg_tac>>gvs[]>>
+  DEP_REWRITE_TAC[encode_eq_sem]>>
+  simp[]>>
+  qpat_x_assum`EVERY _ (FLAT _)` mp_tac>>
+  simp[EVERY_FLAT,MAP_MAP_o,o_DEF,EVERY_MAP]>>
+  simp[Once EVERY_MEM]>>
+  disch_then drule>>
+  simp[]
+QED
+
+Theorem encode_table_sem_2:
+  valid_assignment bnd wi ∧
+  EVERY (λx. iconstraint_sem x (wi,wb)) (encode_table bnd tss Xs) ⇒
+  table_sem tss Xs wi
+Proof
+  simp[encode_table_def,table_sem_def]>>
+  IF_CASES_TAC>>fs[]>>
+  rw[]>>
+  pop_assum mp_tac>>
+  simp[iconstraint_sem_def,MAP_MAP_o,o_DEF,eval_lin_term_def,reify_avar_def,reify_flag_def]>>
+  strip_tac>>
+  first_assum $ irule_at Any>>
+  DEP_REWRITE_TAC [match_row_filter_match]>>
+  CONJ_ASM1_TAC
+  >- fs[EVERY_MEM]>>
+  qpat_x_assum`EVERY _ (FLAT _)` mp_tac>>
+  simp[EVERY_FLAT,MAP_MAP_o,o_DEF,EVERY_MAP]>>
+  simp[Once EVERY_MEM]>>
+  disch_then drule>>
+  metis_tac[reify_tuple_eq_sem]
+QED
+
+Definition encode_extensional_constr_def:
+  encode_extensional_constr bnd c =
+  case c of
+    Table tss Xs =>
+  encode_table bnd tss Xs
+End
+
+Theorem encode_extensional_constr_sem_1:
+  valid_assignment bnd wi ∧
+  extensional_constr_sem c wi ⇒
+  EVERY (λx. iconstraint_sem x (wi,reify_avar wi))
+    (encode_extensional_constr bnd c)
+Proof
+  Cases_on`c`>>
+  rw[encode_extensional_constr_def,extensional_constr_sem_def]>>
+  metis_tac[encode_table_sem_1]
+QED
+
+Theorem encode_extensional_constr_sem_2:
+  valid_assignment bnd wi ∧
+  EVERY (λx. iconstraint_sem x (wi,wb)) (encode_extensional_constr bnd c) ⇒
+  extensional_constr_sem c wi
+Proof
+  Cases_on`c`>>
+  rw[encode_extensional_constr_def,extensional_constr_sem_def]>>
+  metis_tac[encode_table_sem_2]
+QED
+
+Definition cencode_extensional_constr_def:
+  cencode_extensional_constr bnd c pref ec =
+  (ARB:(mlstring option # ciconstraint) app_list,ec:enc_conf)
+End
+
+Theorem cencode_extensional_constr_sem:
+  valid_assignment bnd wi ∧
+  cencode_extensional_constr bnd c pref ec = (es,ec') ⇒
+  ∃fl.
+  enc_rel fl wi es (encode_extensional_constr bnd c) ec ec'
+Proof
+  cheat
+QED
+
+Definition sexp_extensional_constr_def:
+  sexp_extensional_constr name (rest:sexp) =
+    fail (strlit "unsupported constraint: " ^ name)
+End
